easiest fix in a lifetime

Games/gameLib/CountEx_WinStrat.lean
@@ -10,6 +10,14 @@ import Games.gameLib.Termination
 import Games.exLib.List
 
 
+
+def Symm_Game_World.is_fst_win_ALT_0  {α β : Type u} (g : Symm_Game_World α β) : Prop :=
+  ∃ ws : Strategy α β,
+  ∀ snd_s : Strategy α β,
+   (snd_leg : Strategy_legal_snd g.init_game_state g.law ws snd_s ) →
+   (ws_leg : Strategy_legal_fst g.init_game_state g.law ws snd_s) →
+  ({g with fst_strat := ws, fst_lawful := ws_leg, snd_strat := snd_s, snd_lawful := snd_leg} : Symm_Game α β).snd_win
+
 def problem_1 : Symm_Game_World ℕ ℕ where
   init_game_state := 42
   win_states := fun x => x = 0
@@ -17,13 +25,13 @@ def problem_1 : Symm_Game_World ℕ ℕ where
   law := fun _ _ _  => False
 
 
-example : ∃ g : Symm_Game_World ℕ ℕ, g.is_fst_win ∧
+example : ∃ g : Symm_Game_World ℕ ℕ, g.is_fst_win_ALT_0 ∧
   (∀ f_strat s_strat : Strategy ℕ ℕ, ¬ Strategy_legal_fst g.init_game_state g.law f_strat s_strat) :=
   by
   use problem_1
   constructor
   · use (fun _ _ => 666)
-    intro _ nope
+    intro _ _ nope
     exfalso
     dsimp [problem_1] at nope
     specialize nope 0 (by decide)
